Progress on KDF

src/tls/DefineTable.fst
@@ -16,7 +16,7 @@ let alloc #it vt =
     MDM.alloc #it #vt #(fun _ -> True) #tls_define_region ()
   else ()
 
-let extend #it #vt t i k =
+let extend #it #vt t #i k =
   if model then
    begin
     let t0 = ideal t in
@@ -27,32 +27,33 @@ let extend #it #vt t i k =
   else ()
 
 let dt_forall #it #vt t pred h =
-  model ==> (forall (i:it) (k:vt i).
-  {:pattern (defined_as t i k h)}
-  defined_as t i k h ==> pred k h)
+  model ==> (forall (i:it) (k:vt i{defined_as t k h}).
+  {:pattern (defined_as t k h)} pred k h)
 
 val fold_gtot: ('a -> 'b -> GTot 'a) -> 'a -> l:list 'b -> GTot 'a (decreases l)
 let rec fold_gtot f x l = match l with
   | [] -> x
   | hd::tl -> f (fold_gtot f x tl) hd
 
-let fp_add (#it:eqtype) (#vt:it->Type) (#p:M.loc) (fp:local_fp vt p)
-  (l:sub_loc p) (cur:(i:it & vt i)) : GTot (sub_loc p) =
+let fp_add (#it:eqtype) (#vt:it->Type)
+  (fp:local_fp vt) (l:M.loc) (cur:(i:it & vt i)) =
   let (| i, k |) = cur in
   M.loc_union l (fp k)
 
-let footprint #it #vt t #parent fp h =
+let footprint #it #vt t fp h =
   if model then 
     let l = HS.sel h (ideal t) in
     fold_gtot (fp_add fp) M.loc_none l
   else M.loc_none
 
-let lemma_footprint_frame #it #vt t #p fp h0 h1 = ()
+let lemma_footprint_empty #it #vt t fp h0 = ()
 
-let lemma_footprint_extend #it #vt t #p fp i k h0 h1 = ()
+let lemma_footprint_frame #it #vt t fp h0 h1 = ()
+
+let lemma_footprint_extend #it #vt t fp #i k h0 h1 = ()
 
 let rec lemma_fp_includes (#it:eqtype) (vt:it->Type) (t:MDM.map it vt)
-  (#p:M.loc) (fp:local_fp vt p) (i:it) (k:vt i)
+  (fp:local_fp vt) (#i:it) (k:vt i)
   : Lemma (requires (MDM.sel t i == Some k))
   (ensures fold_gtot (fp_add fp) M.loc_none t `M.loc_includes` (fp k))
   (decreases %[t])
@@ -61,104 +62,39 @@ let rec lemma_fp_includes (#it:eqtype) (vt:it->Type) (t:MDM.map it vt)
   | [] -> ()
   | (| x, y |) :: tl ->
     if x = i then ()
-    else lemma_fp_includes vt tl fp i k
+    else lemma_fp_includes vt tl fp k
 
-let lemma_footprint_includes #it #vt t #p fp i k h =
+let lemma_footprint_includes #it #vt t fp #i k h =
   if model then
     let t0 = HS.sel h (ideal t) in
-    lemma_fp_includes vt t0 fp i k
+    lemma_fp_includes vt t0 fp k
   else ()
 
 let lemma_forall_empty #it #vt t pred h = ()
 
-let lemma_forall_elim #it #vt t pred i k h = ()
+let lemma_forall_elim #it #vt t pred h #i k = ()
 
-val lemma_forall_extend_wit:
-  #it: eqtype ->
-  #vt: (it -> Type) ->
-  t: MDM.map it vt ->
-  t': MDM.map it vt ->
-  pred: (#i:it -> vt i -> mem -> GTot Type0) ->
-  #i: it -> k: vt i ->
-  h: mem ->
-  x:it -> y:vt x ->
-  Lemma
-    (requires model /\ pred k h /\
-      ((MDM.sel t x == Some y) ==> pred #x y h) /\
-      t' == (| i, k |) :: t)
-    (ensures (MDM.sel t' x == Some y) ==> pred #x y h)
-
-let lemma_forall_extend_wit #it #vt t t' pred #i k h x y = ()
-
-let lemma_forall_extend #it #vt t pred #p fp pred_frame #i k h0 h1 =
+let lemma_forall_extend #it #vt t pred fp pred_frame #i k h0 h1 =
   if model then
-    let t0 = HS.sel h0 (ideal t) in
-    let t1 = HS.sel h1 (ideal t) in
-    let pred_frame' (#i:it) (k:vt i) (h0:mem) (l:M.loc) (h1:mem)
-      : Lemma ((pred k h0 /\ M.modifies l h0 h1 /\
-        M.loc_disjoint l (fp k)) ==> pred k h1) =
-      FStar.Classical.move_requires (pred_frame k h0 l) h1
-      in
-    let lupd (#x:it) (y:vt x) : Lemma
-      (requires (MDM.sel t0 x == Some y) ==> pred #x y h0)
-      (ensures (MDM.sel t1 x == Some y) ==> pred #x y h1) =
-      assert(MDM.sel t1 x == (if x = i then Some k else MDM.sel t0 x));
+    let prove_on_witness (x:it) (y:vt x{defined_as t y h1})
+      : Lemma (pred y h1) =
       if x = i then ()
-      else pred_frame' #x y h0 (loc t) h1
-      in
-    let prove_on_witness (x:it) (y:vt x)
-      : Lemma (MDM.sel t1 x == Some y ==> pred #x y h1)
-      =
-      lemma_forall_elim t pred x y h0;
-      lupd #x y;
-      lemma_forall_extend_wit t0 t1 pred #i k h1 x y
-      in
+      else (
+        lemma_forall_elim t pred h0 y;
+        lemma_footprint_includes t fp y h0;
+        pred_frame y h0 (loc t) h1
+      ) in
     FStar.Classical.forall_intro_2 prove_on_witness
   else ()
 
-val lemma_forall_frame_wit:
-  #it: eqtype ->
-  #vt: (it -> Type) ->
-  t: dt vt ->
-  pred: (#i:it -> vt i -> mem -> GTot Type0) ->
-  #parent: M.loc ->
-  fp: local_fp vt parent ->
-  pred_frame: (#i:it -> k:vt i -> h0:mem -> l:M.loc -> h1:mem -> Lemma
-    ((pred k h0 /\ M.modifies l h0 h1 /\ M.loc_disjoint l (fp k))
-     ==> pred k h1)) ->
-  h0: mem -> l:M.loc -> h1: mem ->
-  x:it -> y:vt x ->
-  Lemma
-    (requires M.modifies l h0 h1 /\ t `live` h0 /\
-      (defined_as t x y h0 ==> pred y h0) /\
-      M.loc_disjoint l (loc t) /\ M.loc_disjoint l (fp y))
-    (ensures defined_as t x y h1 ==> pred y h1)
-
-let lemma_forall_frame_wit #it #vt t pred #p fp pred_frame h0 l h1 x y =
-  lemma_unchanged_frame t h0 l h1;
-  pred_frame y h0 l h1
-
-// Could be simplified if FStar.Classical had
-// move_requires_2 or forall_impl_intro_2
-let lemma_forall_frame #it #vt t pred #p fp pred_frame h0 l h1 =
+let lemma_forall_frame #it #vt t pred fp pred_frame h0 l h1 =
   if model then 
-    let pred_frame' (#i:it) (k:vt i) (h0:mem) (l:M.loc) (h1:mem)
-      : Lemma ((pred k h0 /\ M.modifies l h0 h1 /\ M.loc_disjoint l (fp k))
-         ==> pred k h1) =
-      FStar.Classical.move_requires (pred_frame k h0 l) h1
-      in
-    let prove_on_witness (v:(i:it & vt i))
-      : Lemma (requires defined_as t (dfst v) (dsnd v) h1)
-        (ensures pred (dsnd v) h1)
+    let prove_on_witness (x:it) (y:vt x{defined_as t y h1})
+      : Lemma (ensures pred y h1)
       =
-      let (| x, y |) = v in
-      lemma_forall_elim t pred x y h0;
-      lemma_footprint_includes t fp x y h0;
-      lemma_forall_frame_wit t pred fp pred_frame' h0 l h1 x y
+      lemma_forall_elim t pred h0 y;
+      lemma_footprint_includes t fp y h0;
+      pred_frame y h0 l h1
       in
-    let prove_on_witness2 (x:it) (y:vt x)
-      : Lemma (defined_as t x y h1 ==> pred y h1)
-      = FStar.Classical.move_requires prove_on_witness (|x,y|)
-      in
-    FStar.Classical.forall_intro_2 prove_on_witness2
+    FStar.Classical.forall_intro_2 prove_on_witness
   else ()
